examples/BabySep.v
@@ -18,8 +18,9 @@ Definition read := bmodule "read" {{
 Theorem readOk : moduleOk read.
   structured; autorewrite with sepFormula in *; simpl in *.
 
-  inBounds_contra.
+  auto.
 
   ho.
-  admit.
+  sepRead.
+  reflexivity.
 Qed.
